

# INTEGRATION AND DIFFERENTIATION

## THE POWER RULE:

The power rule is used to find the first derivative of any function.

If we have a function  $f(x) = x^2$

We can apply the power rule as follows:

If  $f(x) = x^2$   $\rightarrow a = 1$ , so not shown.

$$f'(x) = 2 \times x^{2-1}$$

STEPS: for any function  $f(x) = ax^n$

$$f'(x) = anx^{n-1}$$

another way to write this  
if  $f(x)^n$   
then  $f'(x) = n \times f(x)^{n-1}$

① 1st we times the coefficient of  $x$  by the power ( $n$ )

② then we minus 1 from the power

In our example,  $a = 1$ , so it was not shown.

In short:

$$\text{if } f(x) = x^2$$

$$\text{then } f'(x) = 2x$$

another way of writing it:

$$f(x) = x^2$$

so:

$$f'(x)$$

$$= 2 \times x^{2-1}$$

## REVERSING THE POWER RULE

2

The opposite of deriving is integrating.

So we do the exact opposite in order to get the integral of a function.

$$\text{If } f(x) = 2x$$

- STEPS: ① first add 1 to the exponent 1  
② then divide  $f(x)$  by the a value 2

$$\int 2x \, dx$$

integrate

our example  $f(x)$

with respect to  $x$ .

note that the steps are also reversed in order. The order matters here.

Therefore becomes:

$$\frac{2x^{1+1}}{2}$$

So our formula for reverse power rule is:

$$\int f(x) \, dx = \frac{f(x)^{n+1}}{n+1}$$

note that we are dividing by the new power.

# THE CHAIN RULE (differentiation)

If we take the power rule above, but we have a question with brackets, we can use the chain rule so that we don't have to expand the brackets.

for example if  $f(x) = (3x-2)^4$   
this would take long to expand.

The chain rule states that in this case, for any  $f(x)$ ,  $f'(x)$  is equal to the 1st derivative of outside the bracket times by the first derivative of the contents inside the bracket, like this:

If  $g(x) \rightarrow$  looks like this:  
 $(f(x))^n$

Then:  $g'(x) = n \times (f(x))^{n-1} \times f'(x)$

So using our example:

If  $f(x) = (3x-2)^4$

then  $f'(x) = 4 \times (3x-2)^3 \times 3$

to finish this:  $4 \times 3 = 12$

$12(3x-2)^3$

note that the contents of the bracket are left the same here

this is the 1st derivative of the contents of the bracket.

# REVERSING THE CHAIN RULE: (integration)

4

Just like the power rule, the chain rule is reversible.  
This is used to INTEGRATE.

The reverse chain rule could be shown as follows:

In order to  $\int f(x)^n dx$ , where we have

brackets:

Our integrated function would be found by:

$$\frac{f(x)^{n+1}}{(n+1) \times f'(x)} \rightarrow \text{original plus 1}$$

divide  $n+1$   
instead of  
times to  
reverse it

divide by the  
first derivative of  $f(x)$   
to reverse it.

NOTE: this is again  
the derivative,  
NOT the integral of  
 $f(x)$ .

using our answer as an example:

$$\int 12(3x-2)^3 dx$$

$$= \frac{12(3x-2)^4}{4 \times 3}$$

$$= \frac{12(3x-2)^4}{12} = (3x-2)^4$$

## QUICK VERSION:

### POWER RULE:

$$\text{if } f(x)^n$$

$$\text{then } f'(x) = n \times f(x)^{n-1}$$

### REVERSE POWER RULE:

$$\text{if } \int f(x) dx$$

$$\text{then } \frac{f(x)^{n+1}}{n+1}$$

### CHAIN RULE:

$$\text{if } g(x) \Rightarrow (f(x))^n$$

$$\text{then } g'(x) = n \times (f(x))^{n-1} \times f'(x)$$

### REVERSE CHAIN RULE:

$$\text{if } \int f(x)^n dx \Rightarrow \text{with brackets}$$

$$\text{then } \frac{(f(x))^{n+1}}{(n+1) \times (f'(x))} + C$$

$C$  represents the constant term.  
 this is further explained on the next pg

## WHERE DOES "C" go / come from?

6

When you differentiate  $f(x)$  the constant term falls away.

When you integrate, you need to bring that constant term back.

Ex: If  $f(x) = x^2 + 1$   
 $f'(x) = 2x$

but:

If  $\int 2x \, dx$

we get  $x^2$

So: we are missing the  $+1$

to fix: we  $+c$

If no point given, leave it like this:

$\therefore x^2 + c$

If given:  
sub point  $(1, 2)$

$2 = 1^2 + c$   
 $c = 1$

from here we would need further information to solve for  $c$ , such as subbing in a point on our graph.

↳ This information will be given, or found, on the example, or the function can be left in this form.